Fixed a couple of bugs, added a bunch of debugging vernacs to the examples

src/verit/veritParser.mly
@@ -241,7 +241,7 @@ rulename:
   | TRUE { True }
   | FALSE { Fals }
   | NOTNOT { Notnot }
-  | THRESO { Hole }
+  | THRESO { Hole } /* Needs to be updated */
   | RESO { Reso }
   | TAUT { Taut } /* Needs to be checked */
   | CONT { Cont } /* Needs to be checked */
